v2/unsolved.md
@@ -1,0 +1,10 @@
+* Equiv.v
+- better_subst_equiv
+- ptwice_cequiv_pcopy
+- p3_p4_inequiv
+- p5_p6_equiv
+- Additional Exercices
+
+* Hoare.v
+- hoare_repeat
+- Additional Exercises
